Tests/type_inference/primitive_independent.ml
@@ -1,0 +1,8 @@
+open Mica
+
+let _ =
+  let xs : int list = [] in
+  let ys : bool list = [] in
+  let _ = List.length xs in
+  let _ = List.length ys in
+  ()
